src/SemTy.v
@@ -20,116 +20,93 @@ Section SemTy.
 
 Import ListNotations.
 
-Definition SemPrimType (ty : PrimType) : Type :=
+Definition SemPrimTy (ty : PrimType) : Type :=
   match ty with
+  | PrimUnit    => unit
   | PrimInteger => Z
   | PrimDecimal => N
   | PrimTime    => nat
   | PrimBool    => bool
   | PrimString  => string
-  | PrimUnit    => unit
   end.
-
-Record CapSig : Set := {
-  paramTy : ValueTy;
-  valueTy : ValueTy;
-}.
-
-Derive NoConfusion NoConfusionHom Subterm EqDec for CapSig.
-
-Inductive Cap (s : CapSig) : Set :=
-  | Token (name : string) : Value (paramTy s) → Value (valueTy s) → Cap s.
-
-Derive NoConfusion NoConfusionHom Subterm EqDec for Cap.
-
-Arguments Token {s} name arg val.
-
-Definition nameOf `(c : Cap s) : string :=
-  match c with Token n _ _ => n end.
-
-Definition paramOf `(c : Cap s) : Value (paramTy s) :=
-  match c with Token _ p _ => p end.
-
-Definition valueOf `(c : Cap s) : Value (valueTy s) :=
-  match c with Token _ _ v => v end.
-
-Inductive ACap : Set :=
-  | AToken (s : CapSig) : Cap s → ACap.
-
-Derive NoConfusion NoConfusionHom Subterm EqDec for ACap.
-
-Definition ACap_ext (ac : ACap) : { s : CapSig & Cap s } :=
-  match ac with AToken s c => existT _ s c end.
-
-Arguments Token {s} name arg val.
 
 Context `{Monad m}.
-
-Fixpoint concreteTy (τ : Ty) : ValueTy :=
-  match τ with
-  | ℤ            => TInteger
-  | 𝔻            => TDecimal
-  | 𝕋            => TTime
-  | 𝔹            => TBool
-  | 𝕊            => TString
-  | 𝕌            => TUnit
-  | TySym        => TSymbol
-  | TyList t     => TList (concreteTy t)
-  | TyPair t1 t2 => TPair (concreteTy t1) (concreteTy t2)
-  | _            => TVoid
-  end.
-
-Arguments concreteTy τ /.
 
 Fixpoint SemTy (τ : Ty) : Type :=
   match τ with
   | TyArrow dom cod => SemTy dom → m (SemTy cod)
 
-  | TyCap p v =>
-      Cap {| paramTy := concreteTy p; valueTy := concreteTy v |}
+  | TyPrim p        => SemPrimTy p
+  | TySym           => string
 
-  (* Disallow functions and capabilities from appearing inside data
-     structures. They may only be passed as arguments to functions, or
-     returned from functions. *)
-  | ty              => Value (concreteTy ty)
+  | TyList t        => list (SemTy t)
+  | TyPair t1 t2    => SemTy t1 * SemTy t2
+
+  (* These types are used by capabilities. *)
+  | TyACapList      => list ACap
+  | TyCap p v       => Cap {| paramTy := concreteTy p; valueTy := concreteTy v |}
   end.
 
 Notation "⟦ t ⟧" := (SemTy t) (at level 9) : type_scope.
 
+Equations concrete `(v : ⟦ t ⟧) (C : ConcreteP t) : Value (concreteTy t) :=
+  concrete (t:=𝕌)     v PrimDecP := VUnit;
+  concrete (t:=ℤ)     v PrimDecP := VInteger v;
+  concrete (t:=𝔻)     v PrimDecP := VDecimal v;
+  concrete (t:=𝕋)     v PrimDecP := VTime v;
+  concrete (t:=𝔹)     v PrimDecP := VBool v;
+  concrete (t:=𝕊)     v PrimDecP := VString v;
+  concrete (t:=TySym) v SymDecP  := VSymbol v;
+
+  concrete (t:=TyList _) [] (ListDecP H) := VList [];
+  concrete (t:=TyList _) xs (ListDecP H) := VList (map (λ x, concrete x H) xs);
+
+  concrete (t:=TyPair _ _) (x, y) (PairDecP Hx Hy) :=
+    VPair (concrete x Hx) (concrete y Hy).
+
+Equations reflect `(v : Value (concreteTy t)) : ⟦ t ⟧ :=
+  reflect (t:=TyPrim PrimUnit)    VUnit        := tt;
+  reflect (t:=TyPrim PrimInteger) (VInteger v) := v;
+  reflect (t:=TyPrim PrimDecimal) (VDecimal v) := v;
+  reflect (t:=TyPrim PrimTime)    (VTime v)    := v;
+  reflect (t:=TyPrim PrimBool)    (VBool v)    := v;
+  reflect (t:=TyPrim PrimString)  (VString v)  := v;
+  reflect (t:=TySym)              (VSymbol v)  := v;
+  reflect (t:=TyList _)           (VList vs)   := map reflect vs;
+  reflect (t:=TyPair _ _)         (VPair x y)  := (reflect x, reflect y).
+
+#[export]
+Program Instance SemPrimTy_EqDec {ty} : EqDec (SemPrimTy ty).
+Next Obligation.
+  induction ty; simpl in x, y.
+  - destruct x, y.
+    now left.
+  - apply Z_EqDec.
+  - apply N_EqDec.
+  - apply nat_EqDec.
+  - apply bool_EqDec.
+  - apply string_EqDec.
+Defined.
+
 #[export]
 Program Instance Concrete_EqDec {t} (H : ConcreteP t) : EqDec ⟦t⟧.
 Next Obligation.
-  induction t;
-  first [ now inv H0 | now apply Value_EqDec ].
+  induction H0;
+  try first [ now inv H0 | now apply Value_EqDec ];
+  simpl in x, y.
+  - apply SemPrimTy_EqDec.
+  - apply string_EqDec.
+  - apply list_eqdec.
+    fold SemTy.
+    unfold EqDec.
+    apply IHConcreteP.
+  - destruct x, y.
+    destruct (IHConcreteP1 s s1); subst.
+    + destruct (IHConcreteP2 s0 s2); subst.
+      * now left.
+      * right; intro; now inv H0.
+    + right; intro; now inv H0.
 Defined.
-
-Equations concrete `(v : ⟦ t ⟧) : option (Value (concreteTy t)) :=
-  concrete (t:=TyArrow _ _) v := None;
-  concrete (t:=TyACap)      v := None;
-  concrete (t:=TyCap _ _)   v := None;
-  concrete                  v := Some v.
-
-Equations concreteH `(v : ⟦ t ⟧) (C : ConcreteP t) : Value (concreteTy t) :=
-  concreteH v PrimDecP       := v;
-  concreteH v SymDecP        := v;
-  concreteH v (ListDecP _)   := v;
-  concreteH v (PairDecP _ _) := v.
-
-Equations reflect `(v : Value (concreteTy t)) : ⟦ t ⟧ :=
-  reflect (t:=TyPrim PrimInteger) v := v;
-  reflect (t:=TyPrim PrimDecimal) v := v;
-  reflect (t:=TyPrim PrimTime)    v := v;
-  reflect (t:=TyPrim PrimBool)    v := v;
-  reflect (t:=TyPrim PrimString)  v := v;
-  reflect (t:=TyPrim PrimUnit)    v := v;
-  reflect (t:=TySym)              v := v;
-  reflect (t:=TyList _)           v := v;
-  reflect (t:=TyPair _ _)         v := v.
-
-Definition concreteH1 `{M :Monad m} `(f : ⟦ dom ⟶ cod ⟧) (CC : ConcreteP cod) :
-  Value (concreteTy dom) → m (Value (concreteTy cod)) :=
-  λ x, r <- f (reflect x) ;
-       pure (concreteH r CC).
 
 End SemTy.
 
