src/Exp.v
@@ -80,7 +80,7 @@ Inductive Exp Γ : Ty → Set :=
   | WithCapability {p v τ} :
     ConcreteP p →
     ConcreteP v →
-    Exp Γ (TyCap p v ⟶ TyList TyACap) →
+    Exp Γ (TyCap p v ⟶ TyACapList) →
     Exp Γ (v × v ⟶ v) →
     Exp Γ (TyCap p v) → Exp Γ τ → Exp Γ τ
   | InstallCapability {p v} : Exp Γ (TyCap p v) → Exp Γ 𝕌
