src/Value.v
@@ -87,27 +87,43 @@ Proof.
 Qed.
 
 Inductive ValueTy : Set :=
+  | TVoid
+  | TUnit
+  | TSymbol
   | TInteger
   | TDecimal
   | TTime
   | TBool
   | TString
-  | TUnit
-  | TVoid
-  | TSymbol
   | TList : ValueTy → ValueTy
   | TPair : ValueTy → ValueTy → ValueTy.
 
 Derive NoConfusion NoConfusionHom Subterm EqDec for ValueTy.
 
+Fixpoint concreteTy (τ : Ty) : ValueTy :=
+  match τ with
+  | TySym        => TSymbol
+  | ℤ            => TInteger
+  | 𝔻            => TDecimal
+  | 𝕋            => TTime
+  | 𝔹            => TBool
+  | 𝕊            => TString
+  | 𝕌            => TUnit
+  | TyList t     => TList (concreteTy t)
+  | TyPair t1 t2 => TPair (concreteTy t1) (concreteTy t2)
+  | _            => TVoid
+  end.
+
+Arguments concreteTy τ /.
+
 Inductive Value : ValueTy → Set :=
-  | VInteger      : Z → Value TInteger
-  | VDecimal      : N → Value TDecimal
-  | VTime         : nat → Value TTime
-  | VBool         : bool → Value TBool
-  | VString       : string → Value TString
   | VUnit         : Value TUnit
   | VSymbol       : string → Value TSymbol
+  | VInteger      : Z      → Value TInteger
+  | VDecimal      : N      → Value TDecimal
+  | VTime         : nat    → Value TTime
+  | VBool         : bool   → Value TBool
+  | VString       : string → Value TString
   | VList {t}     : list (Value t) → Value (TList t)
   | VPair {t1 t2} : Value t1 → Value t2 → Value (TPair t1 t2).
 
@@ -136,13 +152,13 @@ Variable Ppair    : ∀ t1 (x : Value t1) t2 (y : Value t2),
 Fixpoint Value_rect' `(e : Value t) : P e.
 Proof.
   induction e.
+  - now apply Punit.
+  - now apply Psym.
   - now apply Pinteger.
   - now apply Pdecimal.
   - now apply Ptime.
   - now apply Pbool.
   - now apply Pstring.
-  - now apply Punit.
-  - now apply Psym.
   - apply Plist.
     induction l.
     * constructor.
@@ -193,6 +209,41 @@ Next Obligation.
     + right; intro.
       now inv H.
 Defined.
+
+(*************************************************************************
+ * Capability values
+ *)
+
+Record CapSig : Set := {
+  paramTy : ValueTy;
+  valueTy : ValueTy;
+}.
+
+Derive NoConfusion NoConfusionHom Subterm EqDec for CapSig.
+
+Inductive Cap (s : CapSig) : Set :=
+  | Token (name : string) : Value (paramTy s) → Value (valueTy s) → Cap s.
+
+Derive NoConfusion NoConfusionHom Subterm EqDec for Cap.
+
+Arguments Token {s} name arg val.
+
+Definition nameOf `(c : Cap s) : string :=
+  match c with Token n _ _ => n end.
+
+Definition paramOf `(c : Cap s) : Value (paramTy s) :=
+  match c with Token _ p _ => p end.
+
+Definition valueOf `(c : Cap s) : Value (valueTy s) :=
+  match c with Token _ _ v => v end.
+
+Inductive ACap : Set :=
+  | AToken (s : CapSig) : Cap s → ACap.
+
+Derive NoConfusion NoConfusionHom Subterm EqDec for ACap.
+
+Definition ACap_ext (ac : ACap) : { s : CapSig & Cap s } :=
+  match ac with AToken s c => existT _ s c end.
 
 End Value.
 
